Finally... it links\!

dist/gcc-compatible/EverCrypt_Poly1305.c
@@ -40,53 +40,9 @@ static void poly1305_vale(uint8_t *dst, uint8_t *src, uint32_t len, uint8_t *key
   else
   {
     uint8_t init = (uint8_t)0U;
+    for (uint32_t i = (uint32_t)0U; i < (uint32_t)16U; i++)
     {
-      tmp[0U] = init;
-    }
-    {
-      tmp[1U] = init;
-    }
-    {
-      tmp[2U] = init;
-    }
-    {
-      tmp[3U] = init;
-    }
-    {
-      tmp[4U] = init;
-    }
-    {
-      tmp[5U] = init;
-    }
-    {
-      tmp[6U] = init;
-    }
-    {
-      tmp[7U] = init;
-    }
-    {
-      tmp[8U] = init;
-    }
-    {
-      tmp[9U] = init;
-    }
-    {
-      tmp[10U] = init;
-    }
-    {
-      tmp[11U] = init;
-    }
-    {
-      tmp[12U] = init;
-    }
-    {
-      tmp[13U] = init;
-    }
-    {
-      tmp[14U] = init;
-    }
-    {
-      tmp[15U] = init;
+      tmp[i] = init;
     }
     uint32_t len16 = n_blocks * (uint32_t)16U;
     uint8_t *src16 = src;
@@ -100,8 +56,6 @@ static void poly1305_vale(uint8_t *dst, uint8_t *src, uint32_t len, uint8_t *key
 
 void EverCrypt_Poly1305_poly1305(uint8_t *dst, uint8_t *src, uint32_t len, uint8_t *key)
 {
-  bool avx2 = EverCrypt_AutoConfig2_has_avx2();
-  bool avx = EverCrypt_AutoConfig2_has_avx();
   bool vec256 = EverCrypt_AutoConfig2_has_vec256();
   bool vec128 = EverCrypt_AutoConfig2_has_vec128();
   #if HACL_CAN_COMPILE_VEC256
