dist/gcc-compatible/Hacl_Chacha20.c
@@ -99,85 +99,11 @@ static inline void chacha20_core(uint32_t *k, uint32_t *ctx, uint32_t ctr)
   uint32_t ctr_u32 = ctr;
   k[12U] = k[12U] + ctr_u32;
   rounds(k);
+  for (uint32_t i = (uint32_t)0U; i < (uint32_t)16U; i++)
   {
     uint32_t *os = k;
-    uint32_t x = k[0U] + ctx[0U];
-    os[0U] = x;
-  }
-  {
-    uint32_t *os = k;
-    uint32_t x = k[1U] + ctx[1U];
-    os[1U] = x;
-  }
-  {
-    uint32_t *os = k;
-    uint32_t x = k[2U] + ctx[2U];
-    os[2U] = x;
-  }
-  {
-    uint32_t *os = k;
-    uint32_t x = k[3U] + ctx[3U];
-    os[3U] = x;
-  }
-  {
-    uint32_t *os = k;
-    uint32_t x = k[4U] + ctx[4U];
-    os[4U] = x;
-  }
-  {
-    uint32_t *os = k;
-    uint32_t x = k[5U] + ctx[5U];
-    os[5U] = x;
-  }
-  {
-    uint32_t *os = k;
-    uint32_t x = k[6U] + ctx[6U];
-    os[6U] = x;
-  }
-  {
-    uint32_t *os = k;
-    uint32_t x = k[7U] + ctx[7U];
-    os[7U] = x;
-  }
-  {
-    uint32_t *os = k;
-    uint32_t x = k[8U] + ctx[8U];
-    os[8U] = x;
-  }
-  {
-    uint32_t *os = k;
-    uint32_t x = k[9U] + ctx[9U];
-    os[9U] = x;
-  }
-  {
-    uint32_t *os = k;
-    uint32_t x = k[10U] + ctx[10U];
-    os[10U] = x;
-  }
-  {
-    uint32_t *os = k;
-    uint32_t x = k[11U] + ctx[11U];
-    os[11U] = x;
-  }
-  {
-    uint32_t *os = k;
-    uint32_t x = k[12U] + ctx[12U];
-    os[12U] = x;
-  }
-  {
-    uint32_t *os = k;
-    uint32_t x = k[13U] + ctx[13U];
-    os[13U] = x;
-  }
-  {
-    uint32_t *os = k;
-    uint32_t x = k[14U] + ctx[14U];
-    os[14U] = x;
-  }
-  {
-    uint32_t *os = k;
-    uint32_t x = k[15U] + ctx[15U];
-    os[15U] = x;
+    uint32_t x = k[i] + ctx[i];
+    os[i] = x;
   }
   k[12U] = k[12U] + ctr_u32;
 }
@@ -190,114 +116,30 @@ chacha20_constants[4U] =
 inline void
 Hacl_Impl_Chacha20_chacha20_init(uint32_t *ctx, uint8_t *k, uint8_t *n, uint32_t ctr)
 {
+  for (uint32_t i = (uint32_t)0U; i < (uint32_t)4U; i++)
   {
     uint32_t *os = ctx;
-    uint32_t x = chacha20_constants[0U];
-    os[0U] = x;
+    uint32_t x = chacha20_constants[i];
+    os[i] = x;
   }
-  {
-    uint32_t *os = ctx;
-    uint32_t x = chacha20_constants[1U];
-    os[1U] = x;
-  }
-  {
-    uint32_t *os = ctx;
-    uint32_t x = chacha20_constants[2U];
-    os[2U] = x;
-  }
-  {
-    uint32_t *os = ctx;
-    uint32_t x = chacha20_constants[3U];
-    os[3U] = x;
-  }
+  for (uint32_t i = (uint32_t)0U; i < (uint32_t)8U; i++)
   {
     uint32_t *os = ctx + (uint32_t)4U;
-    uint8_t *bj = k + (uint32_t)0U * (uint32_t)4U;
+    uint8_t *bj = k + i * (uint32_t)4U;
     uint32_t u = load32_le(bj);
     uint32_t r = u;
     uint32_t x = r;
-    os[0U] = x;
-  }
-  {
-    uint32_t *os = ctx + (uint32_t)4U;
-    uint8_t *bj = k + (uint32_t)1U * (uint32_t)4U;
-    uint32_t u = load32_le(bj);
-    uint32_t r = u;
-    uint32_t x = r;
-    os[1U] = x;
-  }
-  {
-    uint32_t *os = ctx + (uint32_t)4U;
-    uint8_t *bj = k + (uint32_t)2U * (uint32_t)4U;
-    uint32_t u = load32_le(bj);
-    uint32_t r = u;
-    uint32_t x = r;
-    os[2U] = x;
-  }
-  {
-    uint32_t *os = ctx + (uint32_t)4U;
-    uint8_t *bj = k + (uint32_t)3U * (uint32_t)4U;
-    uint32_t u = load32_le(bj);
-    uint32_t r = u;
-    uint32_t x = r;
-    os[3U] = x;
-  }
-  {
-    uint32_t *os = ctx + (uint32_t)4U;
-    uint8_t *bj = k + (uint32_t)4U * (uint32_t)4U;
-    uint32_t u = load32_le(bj);
-    uint32_t r = u;
-    uint32_t x = r;
-    os[4U] = x;
-  }
-  {
-    uint32_t *os = ctx + (uint32_t)4U;
-    uint8_t *bj = k + (uint32_t)5U * (uint32_t)4U;
-    uint32_t u = load32_le(bj);
-    uint32_t r = u;
-    uint32_t x = r;
-    os[5U] = x;
-  }
-  {
-    uint32_t *os = ctx + (uint32_t)4U;
-    uint8_t *bj = k + (uint32_t)6U * (uint32_t)4U;
-    uint32_t u = load32_le(bj);
-    uint32_t r = u;
-    uint32_t x = r;
-    os[6U] = x;
-  }
-  {
-    uint32_t *os = ctx + (uint32_t)4U;
-    uint8_t *bj = k + (uint32_t)7U * (uint32_t)4U;
-    uint32_t u = load32_le(bj);
-    uint32_t r = u;
-    uint32_t x = r;
-    os[7U] = x;
+    os[i] = x;
   }
   ctx[12U] = ctr;
+  for (uint32_t i = (uint32_t)0U; i < (uint32_t)3U; i++)
   {
     uint32_t *os = ctx + (uint32_t)13U;
-    uint8_t *bj = n + (uint32_t)0U * (uint32_t)4U;
+    uint8_t *bj = n + i * (uint32_t)4U;
     uint32_t u = load32_le(bj);
     uint32_t r = u;
     uint32_t x = r;
-    os[0U] = x;
-  }
-  {
-    uint32_t *os = ctx + (uint32_t)13U;
-    uint8_t *bj = n + (uint32_t)1U * (uint32_t)4U;
-    uint32_t u = load32_le(bj);
-    uint32_t r = u;
-    uint32_t x = r;
-    os[1U] = x;
-  }
-  {
-    uint32_t *os = ctx + (uint32_t)13U;
-    uint8_t *bj = n + (uint32_t)2U * (uint32_t)4U;
-    uint32_t u = load32_le(bj);
-    uint32_t r = u;
-    uint32_t x = r;
-    os[2U] = x;
+    os[i] = x;
   }
 }
 
@@ -312,261 +154,24 @@ Hacl_Impl_Chacha20_chacha20_encrypt_block(
   uint32_t k[16U] = { 0U };
   chacha20_core(k, ctx, incr);
   uint32_t bl[16U] = { 0U };
+  for (uint32_t i = (uint32_t)0U; i < (uint32_t)16U; i++)
   {
     uint32_t *os = bl;
-    uint8_t *bj = text + (uint32_t)0U * (uint32_t)4U;
+    uint8_t *bj = text + i * (uint32_t)4U;
     uint32_t u = load32_le(bj);
     uint32_t r = u;
     uint32_t x = r;
-    os[0U] = x;
+    os[i] = x;
   }
+  for (uint32_t i = (uint32_t)0U; i < (uint32_t)16U; i++)
   {
     uint32_t *os = bl;
-    uint8_t *bj = text + (uint32_t)1U * (uint32_t)4U;
-    uint32_t u = load32_le(bj);
-    uint32_t r = u;
-    uint32_t x = r;
-    os[1U] = x;
+    uint32_t x = bl[i] ^ k[i];
+    os[i] = x;
   }
+  for (uint32_t i = (uint32_t)0U; i < (uint32_t)16U; i++)
   {
-    uint32_t *os = bl;
-    uint8_t *bj = text + (uint32_t)2U * (uint32_t)4U;
-    uint32_t u = load32_le(bj);
-    uint32_t r = u;
-    uint32_t x = r;
-    os[2U] = x;
-  }
-  {
-    uint32_t *os = bl;
-    uint8_t *bj = text + (uint32_t)3U * (uint32_t)4U;
-    uint32_t u = load32_le(bj);
-    uint32_t r = u;
-    uint32_t x = r;
-    os[3U] = x;
-  }
-  {
-    uint32_t *os = bl;
-    uint8_t *bj = text + (uint32_t)4U * (uint32_t)4U;
-    uint32_t u = load32_le(bj);
-    uint32_t r = u;
-    uint32_t x = r;
-    os[4U] = x;
-  }
-  {
-    uint32_t *os = bl;
-    uint8_t *bj = text + (uint32_t)5U * (uint32_t)4U;
-    uint32_t u = load32_le(bj);
-    uint32_t r = u;
-    uint32_t x = r;
-    os[5U] = x;
-  }
-  {
-    uint32_t *os = bl;
-    uint8_t *bj = text + (uint32_t)6U * (uint32_t)4U;
-    uint32_t u = load32_le(bj);
-    uint32_t r = u;
-    uint32_t x = r;
-    os[6U] = x;
-  }
-  {
-    uint32_t *os = bl;
-    uint8_t *bj = text + (uint32_t)7U * (uint32_t)4U;
-    uint32_t u = load32_le(bj);
-    uint32_t r = u;
-    uint32_t x = r;
-    os[7U] = x;
-  }
-  {
-    uint32_t *os = bl;
-    uint8_t *bj = text + (uint32_t)8U * (uint32_t)4U;
-    uint32_t u = load32_le(bj);
-    uint32_t r = u;
-    uint32_t x = r;
-    os[8U] = x;
-  }
-  {
-    uint32_t *os = bl;
-    uint8_t *bj = text + (uint32_t)9U * (uint32_t)4U;
-    uint32_t u = load32_le(bj);
-    uint32_t r = u;
-    uint32_t x = r;
-    os[9U] = x;
-  }
-  {
-    uint32_t *os = bl;
-    uint8_t *bj = text + (uint32_t)10U * (uint32_t)4U;
-    uint32_t u = load32_le(bj);
-    uint32_t r = u;
-    uint32_t x = r;
-    os[10U] = x;
-  }
-  {
-    uint32_t *os = bl;
-    uint8_t *bj = text + (uint32_t)11U * (uint32_t)4U;
-    uint32_t u = load32_le(bj);
-    uint32_t r = u;
-    uint32_t x = r;
-    os[11U] = x;
-  }
-  {
-    uint32_t *os = bl;
-    uint8_t *bj = text + (uint32_t)12U * (uint32_t)4U;
-    uint32_t u = load32_le(bj);
-    uint32_t r = u;
-    uint32_t x = r;
-    os[12U] = x;
-  }
-  {
-    uint32_t *os = bl;
-    uint8_t *bj = text + (uint32_t)13U * (uint32_t)4U;
-    uint32_t u = load32_le(bj);
-    uint32_t r = u;
-    uint32_t x = r;
-    os[13U] = x;
-  }
-  {
-    uint32_t *os = bl;
-    uint8_t *bj = text + (uint32_t)14U * (uint32_t)4U;
-    uint32_t u = load32_le(bj);
-    uint32_t r = u;
-    uint32_t x = r;
-    os[14U] = x;
-  }
-  {
-    uint32_t *os = bl;
-    uint8_t *bj = text + (uint32_t)15U * (uint32_t)4U;
-    uint32_t u = load32_le(bj);
-    uint32_t r = u;
-    uint32_t x = r;
-    os[15U] = x;
-  }
-  {
-    uint32_t *os = bl;
-    uint32_t x = bl[0U] ^ k[0U];
-    os[0U] = x;
-  }
-  {
-    uint32_t *os = bl;
-    uint32_t x = bl[1U] ^ k[1U];
-    os[1U] = x;
-  }
-  {
-    uint32_t *os = bl;
-    uint32_t x = bl[2U] ^ k[2U];
-    os[2U] = x;
-  }
-  {
-    uint32_t *os = bl;
-    uint32_t x = bl[3U] ^ k[3U];
-    os[3U] = x;
-  }
-  {
-    uint32_t *os = bl;
-    uint32_t x = bl[4U] ^ k[4U];
-    os[4U] = x;
-  }
-  {
-    uint32_t *os = bl;
-    uint32_t x = bl[5U] ^ k[5U];
-    os[5U] = x;
-  }
-  {
-    uint32_t *os = bl;
-    uint32_t x = bl[6U] ^ k[6U];
-    os[6U] = x;
-  }
-  {
-    uint32_t *os = bl;
-    uint32_t x = bl[7U] ^ k[7U];
-    os[7U] = x;
-  }
-  {
-    uint32_t *os = bl;
-    uint32_t x = bl[8U] ^ k[8U];
-    os[8U] = x;
-  }
-  {
-    uint32_t *os = bl;
-    uint32_t x = bl[9U] ^ k[9U];
-    os[9U] = x;
-  }
-  {
-    uint32_t *os = bl;
-    uint32_t x = bl[10U] ^ k[10U];
-    os[10U] = x;
-  }
-  {
-    uint32_t *os = bl;
-    uint32_t x = bl[11U] ^ k[11U];
-    os[11U] = x;
-  }
-  {
-    uint32_t *os = bl;
-    uint32_t x = bl[12U] ^ k[12U];
-    os[12U] = x;
-  }
-  {
-    uint32_t *os = bl;
-    uint32_t x = bl[13U] ^ k[13U];
-    os[13U] = x;
-  }
-  {
-    uint32_t *os = bl;
-    uint32_t x = bl[14U] ^ k[14U];
-    os[14U] = x;
-  }
-  {
-    uint32_t *os = bl;
-    uint32_t x = bl[15U] ^ k[15U];
-    os[15U] = x;
-  }
-  {
-    store32_le(out + (uint32_t)0U * (uint32_t)4U, bl[0U]);
-  }
-  {
-    store32_le(out + (uint32_t)1U * (uint32_t)4U, bl[1U]);
-  }
-  {
-    store32_le(out + (uint32_t)2U * (uint32_t)4U, bl[2U]);
-  }
-  {
-    store32_le(out + (uint32_t)3U * (uint32_t)4U, bl[3U]);
-  }
-  {
-    store32_le(out + (uint32_t)4U * (uint32_t)4U, bl[4U]);
-  }
-  {
-    store32_le(out + (uint32_t)5U * (uint32_t)4U, bl[5U]);
-  }
-  {
-    store32_le(out + (uint32_t)6U * (uint32_t)4U, bl[6U]);
-  }
-  {
-    store32_le(out + (uint32_t)7U * (uint32_t)4U, bl[7U]);
-  }
-  {
-    store32_le(out + (uint32_t)8U * (uint32_t)4U, bl[8U]);
-  }
-  {
-    store32_le(out + (uint32_t)9U * (uint32_t)4U, bl[9U]);
-  }
-  {
-    store32_le(out + (uint32_t)10U * (uint32_t)4U, bl[10U]);
-  }
-  {
-    store32_le(out + (uint32_t)11U * (uint32_t)4U, bl[11U]);
-  }
-  {
-    store32_le(out + (uint32_t)12U * (uint32_t)4U, bl[12U]);
-  }
-  {
-    store32_le(out + (uint32_t)13U * (uint32_t)4U, bl[13U]);
-  }
-  {
-    store32_le(out + (uint32_t)14U * (uint32_t)4U, bl[14U]);
-  }
-  {
-    store32_le(out + (uint32_t)15U * (uint32_t)4U, bl[15U]);
+    store32_le(out + i * (uint32_t)4U, bl[i]);
   }
 }
 
