dist/gcc-compatible/Hacl_Chacha20Poly1305_32.c
@@ -585,68 +585,9 @@ Hacl_Chacha20Poly1305_32_aead_decrypt(
   uint8_t *key = tmp;
   poly1305_do_32(key, aadlen, aad, mlen, cipher, computed_mac);
   uint8_t res = (uint8_t)255U;
+  for (uint32_t i = (uint32_t)0U; i < (uint32_t)16U; i++)
   {
-    uint8_t uu____0 = FStar_UInt8_eq_mask(computed_mac[0U], mac[0U]);
-    res = uu____0 & res;
-  }
-  {
-    uint8_t uu____0 = FStar_UInt8_eq_mask(computed_mac[1U], mac[1U]);
-    res = uu____0 & res;
-  }
-  {
-    uint8_t uu____0 = FStar_UInt8_eq_mask(computed_mac[2U], mac[2U]);
-    res = uu____0 & res;
-  }
-  {
-    uint8_t uu____0 = FStar_UInt8_eq_mask(computed_mac[3U], mac[3U]);
-    res = uu____0 & res;
-  }
-  {
-    uint8_t uu____0 = FStar_UInt8_eq_mask(computed_mac[4U], mac[4U]);
-    res = uu____0 & res;
-  }
-  {
-    uint8_t uu____0 = FStar_UInt8_eq_mask(computed_mac[5U], mac[5U]);
-    res = uu____0 & res;
-  }
-  {
-    uint8_t uu____0 = FStar_UInt8_eq_mask(computed_mac[6U], mac[6U]);
-    res = uu____0 & res;
-  }
-  {
-    uint8_t uu____0 = FStar_UInt8_eq_mask(computed_mac[7U], mac[7U]);
-    res = uu____0 & res;
-  }
-  {
-    uint8_t uu____0 = FStar_UInt8_eq_mask(computed_mac[8U], mac[8U]);
-    res = uu____0 & res;
-  }
-  {
-    uint8_t uu____0 = FStar_UInt8_eq_mask(computed_mac[9U], mac[9U]);
-    res = uu____0 & res;
-  }
-  {
-    uint8_t uu____0 = FStar_UInt8_eq_mask(computed_mac[10U], mac[10U]);
-    res = uu____0 & res;
-  }
-  {
-    uint8_t uu____0 = FStar_UInt8_eq_mask(computed_mac[11U], mac[11U]);
-    res = uu____0 & res;
-  }
-  {
-    uint8_t uu____0 = FStar_UInt8_eq_mask(computed_mac[12U], mac[12U]);
-    res = uu____0 & res;
-  }
-  {
-    uint8_t uu____0 = FStar_UInt8_eq_mask(computed_mac[13U], mac[13U]);
-    res = uu____0 & res;
-  }
-  {
-    uint8_t uu____0 = FStar_UInt8_eq_mask(computed_mac[14U], mac[14U]);
-    res = uu____0 & res;
-  }
-  {
-    uint8_t uu____0 = FStar_UInt8_eq_mask(computed_mac[15U], mac[15U]);
+    uint8_t uu____0 = FStar_UInt8_eq_mask(computed_mac[i], mac[i]);
     res = uu____0 & res;
   }
   uint8_t z = res;
