code/blake2/Hacl.Impl.Blake2.Core.fst
@@ -354,6 +354,7 @@ let load_state_from_state32 #a #m st st32 =
     assert (state_v h1 st == state_v h0 st32)
 #pop-options
 
+
 #push-options "--z3rlimit 100"
 let store_state_to_state32 #a #m st32 st =
     let r0 = rowi st 0ul in
@@ -388,3 +389,4 @@ let store_state_to_state32 #a #m st32 st =
     Lib.Sequence.eq_intro (as_seq h1 b3) (Spec.load_row #a (as_seq h1 b3));
     assert (state_v h1 st32 == state_v h0 st)
 #pop-options
+
